\documentclass[a4paper]{article}
\usepackage{amsmath,amssymb,amsthm,tikz,hyperref}

\newtheorem{exercise}{Exercise}[subsection]

\newcommand*{\E}{\mathbb{E}}
\newcommand*{\R}{\mathbb{R}}
\newcommand*{\cN}{\mathcal{N}}

\renewcommand{\theenumi}{(\alph{enumi})}
\makeatletter

\newenvironment{customExercise}[1]
 {\count@\c@exercise
 \global\c@exercise#1 %
   \global\advance\c@exercise\m@ne
   \exercise}
  {\endexercise
  \global\c@exercise\count@}

\title{Appetizer}
\author{Taeyoung Kim}
\date{\today}

\begin{document}
\maketitle

\setcounter{section}{0}
\setcounter{subsection}{0}


\begin{customExercise}{3}
  Check the following variance identities.
  \begin{enumerate}
    \item Let $Z_1, \ldots, Z_k$ be independent mean-zero random vectors in $\R^n$. Show that
    \[\E\left\| \sum_{j=1}^k Z_j \right\|_2^2 = \sum_{j=1}^k \E\left\| Z_j \right\|_2^2.\]
    \item Let $Z$ be a random vector in $\R^n$. Show that
    \[\E\|Z - \E Z\|_2^2 = \E \|Z\|_2^2 - \|\E Z\|_2^2.\]
  \end{enumerate}
\end{customExercise}
\begin{proof}
  \begin{enumerate}
    \item 
    \begin{align*}
      \E \left\|\sum_{j=1}^k Z_j\right\|_2^2 
      &= \E \left[ \sum_{d=1}^n \left( \sum_{j=1}^k Z_{j,d} \right)^2 \right] &\text{By def.}
      \\
      &= \sum_{d=1}^n \E \left[ \left( \sum_{j=1}^k Z_{j,d} \right)^2 \right] &\text{By lin. of exp.}
      \\
      &= \sum_{d=1}^n \E \left[ \sum_{j=1}^k Z_{j,d}^2 + \sum_{\substack{j,l = 1\\j \neq l}}^k Z_{j,d} Z_{l,d} \right] &\text{Unroll square}
      \\
      &= \sum_{d=1}^n \E \left[ \sum_{j=1}^k Z_{j,d}^2 \right] &\text{Indep. + Zero Mean}
      \\
      &= \sum_{j=1}^k \E \left[ \sum_{d=1}^n Z_{j,d}^2 \right] &\text{By lin. of exp.}
      \\
      &= \sum_{j=1}^k \E \left\| Z_j \right\|^2. &\text{By def.}
    \end{align*}
    \item For conveneice, denote $\mu = \E Z$.
    \begin{align*}
      \E \|Z - \mu\|_2^2 &= \E \left[ \sum_{d=1}^n (Z_d - \mu_d)^2 \right] &\text{By def.}
      \\
      &= \sum_{d=1}^n \E \left[ (Z_d - \mu_d)^2 \right] &\text{By lin. of exp.}
      \\
      &= \sum_{d=1}^n \E \left[ Z_d^2 - 2 Z_d \mu_d + \mu_d^2 \right] &\text{Unroll square}
      \\
      &= \sum_{d=1}^n \E \left[ Z_d^2 - \mu_d^2 \right] &\text{Use } \E Z_d = \mu_d
      \\
      &= \E\|Z\|_2^2 - \|\E Z\|_2^2.
    \end{align*}
  \end{enumerate}
\end{proof}

\begin{customExercise}{5}
  Prove the inequalities
  \[\left(\frac{n}{m}\right)^m \le \binom{n}{m} \le \sum_{k=0}^m \binom{n}{k} \le \left( \frac{en}{m} \right)^m\]
  for all $m \in [1, n]$.
\end{customExercise}
\begin{proof}
  We can rewrite the first inequality as
  \[
    \frac{m}{m} \cdot \frac{m-1}{m} \cdot \ldots \cdot \frac{1}{m} \le \frac{n}{n} \cdot \frac{n-1}{n} \cdot \ldots \cdot \frac{n-m+1}{n}
  \]
  We can pair them by order, and can see that all the terms in the RHS are larger than or equal to terms in LHS. So the first inequality holds.

  Second inequality is immediate, since
  \[\sum_{k=0}^m \binom{n}{k} = \sum_{k=0}^{m-1} \binom{n}{k} + \binom{n}{m}.\]

  For the final inequality, we can show it as
  \begin{align*}
    \sum_{k=0}^m \binom{n}{k} 
    &= \sum_{k=0}^m \frac{n \cdot (n-1) \cdot \ldots \cdot (n-k+1)}{k!} 
    \\
    &\le \sum_{k=0}^m \frac{n^k}{k!}
    \\
    &= \sum_{k=0}^m \frac{m^k}{k!} \left( \frac{n}{m} \right)^k
    \\
    &\le \left(\frac{n}{m}\right)^m \sum_{k=0}^m \frac{m^k}{k!}
    \\
    &\le \left(\frac{n}{m}\right)^m \sum_{k=0}^\infty \frac{m^k}{k!}
    \\
    &= \left( \frac{en}{m} \right)^m.
  \end{align*}
\end{proof}

\begin{customExercise}{6}
  Check that, in Corollary 0.0.4, 
  \[
    (C+C \epsilon^2 N)^{\lceil 1/\epsilon^2 \rceil}
  \]
  Euclidean balls suffice. Here $C$ is a suitable absolute constant.
\end{customExercise}
\begin{proof}
  By simple combinatoric argument, we can explicitly compute that 
  \[|\cN| = \binom{N + k - 1}{k}.\]
  And by our previous exercise, we can bound this value by
  \[|\cN| \le \left( \frac{e(N+k-1)}{k} \right)^k.\]
  Using the fact that $k = \lceil 1/\epsilon^2 \rceil$
  \begin{align*}
    |\cN| 
    &\le \left( e \epsilon^2 N + (k-1)\epsilon^2 \right)^{\lceil 1/\epsilon^2 \rceil} 
    \\
    &\le \left( e \epsilon^2 N ((1 + 1/\epsilon^2) - 1)\epsilon^2 \right)^{\lceil 1/\epsilon^2 \rceil} 
    \\
    &= \left( e \epsilon^2 N + 1 \right)^{\lceil 1/\epsilon^2 \rceil}.
  \end{align*}
\end{proof}
\end{document}